src/GoSep.v
@@ -28,7 +28,7 @@ Definition mem_of := ((fun m k => VarMap.find k m) : locals -> @Mem.mem var Nat.
 Notation "m ≲ p" := (mem_of m ## p * any) (at level 70).
 
 
-Notation "k ~>? t" := (exists val, k |-> Val t val)%pred (at level 35) : pred_scope.
+Notation "k ~>? T" := (exists val, k |-> Val (@wrap_type T _) val)%pred (at level 35) : pred_scope.
 
 Module VarMapFacts := FMapFacts.WFacts_fun(Nat_as_OT)(VarMap).
 
